some fixing

Iris/Iris/BI/Lib/Fractional.lean
@@ -27,6 +27,8 @@ section Divide
 variable {PROP : Type _} [BI PROP]
 open BI.BigSepL
 
+-- TODO: Fix this section to adapt to the new Qp changes
+
 theorem fractional_bigSepL_replicate {Φ : Qp → PROP} [Fractional Φ] (r : Qp) :
     ∀ (k : Nat) (q : Qp), q.1 = ((k : Rat) + 1) * r.1 →
     (Φ q ⊢ [∗list] _x ∈ List.replicate (k + 1) r, Φ r) := by
@@ -40,21 +42,31 @@ theorem fractional_bigSepL_replicate {Φ : Qp → PROP} [Fractional Φ] (r : Qp)
     intro q hq
     have hpos : (0 : Rat) < ((k : Rat) + 1) * r.1 := Rat.mul_pos (by grind) r.2
     have hlt : r < q := by show r.1 < q.1; grind
-    obtain ⟨c, hc⟩ := NumericFraction.lt_def.mp hlt
+    obtain ⟨c, hc⟩ : ∃ c,  r + c = q := sorry
+    -- obtain ⟨c, hc⟩ := NumericFraction.lt_def.mp hlt
     have hcval : c.1 = ((k : Rat) + 1) * r.1 := by
-      have hrc : r.1 + c.1 = q.1 := congrArg Subtype.val hc
+      have hrc : r.1 + c.1 = q.1 := sorry -- congrArg Subtype.val hc
       grind
     rw [← hc, List.replicate_succ]
     exact ((Fractional.fractional r c).1.trans (sep_mono_right (ih c hcval))).trans
       (bigSepL_cons (Φ := fun _ _ => Φ r) (x := r) (xs := List.replicate (k + 1) r)).2
 
+/-- The number q / n -/
+def Rat.divide_even (q : Rat) (n : Nat) : Rat :=
+  q.div n
+
+def Qp.divide_even (q : Qp) (n : Nat) (Hn : 0 < n) : Qp where
+  val := q.1.div n
+  property := sorry
+
 theorem fractional_divide_equal {Φ : Qp → PROP} [Fractional Φ] (q : Qp) (n : Nat) :
-    Φ q ⊢ [∗list] _x ∈ List.replicate (n + 1) (q.div (Qp.ofPNat (n + 1) (Nat.succ_pos n))),
-      Φ (q.div (Qp.ofPNat (n + 1) (Nat.succ_pos n))) := by
+    Φ q ⊢ [∗list] _x ∈ List.replicate (n + 1) (q.divide_even (n+1) (by grind)),
+      Φ (q.divide_even (n+1) (by grind)) := by
   apply fractional_bigSepL_replicate
-  have h := Qp.ofPNat_mul_div q (n + 1) (Nat.succ_pos n)
-  have hof : (Qp.ofPNat (n + 1) (Nat.succ_pos n)).1 = (n : Rat) + 1 := by
-    show ((n + 1 : Nat) : Rat) = (n : Rat) + 1; grind
-  grind
+  sorry
+  -- have h := Qp.ofPNat_mul_div q (n + 1) (Nat.succ_pos n)
+  -- have hof : (Qp.ofPNat (n + 1) (Nat.succ_pos n)).1 = (n : Rat) + 1 := by
+  --   show ((n + 1 : Nat) : Rat) = (n : Rat) + 1; grind
+  -- grind
 
 end Divide
